theories/RTac/AtGoal.v
@@ -11,26 +11,22 @@ Set Strict Implicit.
 Section parameterized.
   Variable typ : Type.
   Variable expr : Type.
-  Variable subst : Type.
 
   Context {RType_typ : RType typ}.
   Context {Expr_expr : Expr RType_typ expr}.
   Context {Typ0_Prop : Typ0 _ Prop}.
-  Context {Subst_subst : Subst subst expr}.
-  Context {SubstOk_subst : @SubstOk _ _ _ _ Expr_expr Subst_subst}.
 
   Variable tac
-  : forall ctx : Ctx typ expr, ctx_subst subst ctx -> expr
-                               -> rtac typ expr subst.
+  : forall ctx : Ctx typ expr, ctx_subst ctx -> expr
+                               -> rtac typ expr.
 
   Definition AT_GOAL
-  : rtac typ expr subst :=
+  : rtac typ expr :=
     fun tus tvs nus nvs ctx s e => (@tac ctx s e) tus tvs nus nvs ctx s e.
 
-  Variables tus tvs : tenv typ.
-  Hypothesis tac_sound : forall c s e, rtac_sound tus tvs (@tac c s e).
+  Hypothesis tac_sound : forall c s e, rtac_sound (@tac c s e).
 
-  Theorem AT_GOAL_sound : rtac_sound tus tvs AT_GOAL.
+  Theorem AT_GOAL_sound : rtac_sound AT_GOAL.
   Proof.
     unfold AT_GOAL; simpl.
     red. intros; subst.
