theories/RTac/First.v
@@ -9,17 +9,13 @@ Set Strict Implicit.
 Section parameterized.
   Variable typ : Type.
   Variable expr : Type.
-  Variable subst : Type.
 
   Context {RType_typ : RType typ}.
   Context {Expr_expr : Expr RType_typ expr}.
   Context {Typ0_Prop : Typ0 _ Prop}.
-  Context {Subst_subst : Subst subst expr}.
-  Context {SubstUpdate_subst : SubstUpdate subst expr}.
-  Context {SubstOk_subst : @SubstOk _ _ _ _ Expr_expr Subst_subst}.
 
-  Fixpoint FIRST (tacs : list (rtac typ expr subst))
-  : rtac typ expr subst :=
+  Fixpoint FIRST (tacs : list (rtac typ expr))
+  : rtac typ expr :=
     fun tus tvs nus nvs ctx s gl =>
       match tacs with
         | nil => Fail
@@ -31,15 +27,15 @@ Section parameterized.
       end.
 
   Theorem FIRST_sound
-  : forall tus tvs tacs, Forall (rtac_sound tus tvs) tacs -> rtac_sound tus tvs (FIRST tacs).
+  : forall tacs, Forall (rtac_sound) tacs -> rtac_sound (FIRST tacs).
   Proof.
     unfold FIRST.
     induction 1.
     { unfold rtac_sound. intros; subst; simpl; auto. }
     { red. intros.
       specialize (H ctx s g _ eq_refl).
-      subst. destruct (x (tus ++ getUVars ctx) (tvs ++ getVars ctx)
-         (length (tus ++ getUVars ctx)) (length (tvs ++ getVars ctx)) ctx s g); eauto. }
+      subst. destruct (x (getUVars ctx) (getVars ctx)
+         (length (getUVars ctx)) (length (getVars ctx)) ctx s g); eauto. }
   Qed.
 
 End parameterized.
