theories/RTac/Solve.v
@@ -9,15 +9,11 @@ Set Strict Implicit.
 Section parameterized.
   Context {typ : Type}.
   Context {expr : Type}.
-  Context {subst : Type}.
   Context {RType_typ : RType typ}.
   Context {Expr_expr : Expr RType_typ expr}.
   Context {Typ0_Prop : Typ0 _ Prop}.
-  Context {Subst_subst : Subst subst expr}.
-  Context {SubstUpdate_subst : SubstUpdate subst expr}.
-  Context {SubstOk_subst : @SubstOk _ _ _ _ Expr_expr Subst_subst}.
 
-  Definition SOLVE (tac : rtac typ expr subst) : rtac typ expr subst :=
+  Definition SOLVE (tac : rtac typ expr) : rtac typ expr :=
     fun tus tvs nus nvs ctx s g =>
       match tac tus tvs nus nvs ctx s g with
         | Solved s => Solved s
@@ -25,13 +21,13 @@ Section parameterized.
       end.
 
   Theorem SOLVE_sound
-  : forall tus tvs tac, rtac_sound tus tvs tac -> rtac_sound tus tvs (SOLVE tac).
+  : forall tac, rtac_sound tac -> rtac_sound (SOLVE tac).
   Proof.
     unfold SOLVE, rtac_sound.
     intros.
     specialize (H ctx s g).
-    subst; destruct (tac (tus ++ getUVars ctx) (tvs ++ getVars ctx)
-           (length (tus ++ getUVars ctx)) (length (tvs ++ getVars ctx)) ctx s g); auto.
+    subst; destruct (tac (getUVars ctx) (getVars ctx)
+           (length (getUVars ctx)) (length (getVars ctx)) ctx s g); auto.
     specialize (H _ eq_refl).
     eapply rtac_spec_Fail.
   Qed.
