theories/RTac/Then.v
@@ -10,19 +10,14 @@ Set Strict Implicit.
 Section parameterized.
   Variable typ : Type.
   Variable expr : Type.
-  Variable subst : Type.
 
   Context {RType_typ : RType typ}.
   Context {Expr_expr : Expr RType_typ expr}.
   Context {Typ0_Prop : Typ0 _ Prop}.
-  Context {Subst_subst : Subst subst expr}.
-  Context {SubstOk_subst : @SubstOk _ _ _ _ Expr_expr Subst_subst}.
-  Context {SubstUpdate_subst : SubstUpdate subst expr}.
-  Context {SubstUpdateOk_subst : SubstUpdateOk _ _}.
 
-  Definition THEN (c1 : rtac typ expr subst)
-             (c2 : rtacK typ expr subst)
-  : rtac typ expr subst :=
+  Definition THEN (c1 : rtac typ expr)
+             (c2 : rtacK typ expr)
+  : rtac typ expr :=
     fun tus tvs nus nvs ctx sub g =>
       match c1 tus tvs nus nvs ctx sub g with
         | More_ sub' g' => c2 tus tvs nus nvs _ sub' g'
@@ -31,11 +26,10 @@ Section parameterized.
       end.
 
   Theorem THEN_sound
-  : forall (tus tvs : list typ) (tac1 : rtac typ expr subst)
-                                (tac2 : rtacK typ expr subst),
-      rtac_sound tus tvs tac1 ->
-      rtacK_sound tus tvs tac2 ->
-      rtac_sound tus tvs (THEN tac1 tac2).
+  : forall (tac1 : rtac typ expr) (tac2 : rtacK typ expr),
+      rtac_sound tac1 ->
+      rtacK_sound tac2 ->
+      rtac_sound (THEN tac1 tac2).
   Proof.
     unfold THEN.
     intros.
